examples/map/MapMAproof.v
@@ -1,5 +1,5 @@
 Require Import Coqlib ITreelib sflib.
-Require Import MapHeader MapM MapA SMod ModSim.
+Require Import MapHeader MapM MapA MapMSpec MapASpec SMod ModSim.
 Require Import ImpPrelude.
 Require Import Skeleton.
 Require Import PCM IPM.
@@ -31,23 +31,25 @@ Set Implicit Arguments.
 
 Local Open Scope nat_scope.
 
-
-
+Module MapMA.
 Section SIMMODSEM.
-  Context `{_M: MapRA.t}.
-  Context `{@GRA.inG memRA Γ}. 
+  Context `{_W: CtxWD.t}.
+  Context `{_M: MapMR.t (Γ:=Γ)}.
+  Context `{_A: MapAR.t (Γ:=Γ)}.
 
+  Import MapAS.
+  
   Section LEMMA. 
-    Local Transparent unallocated map_points_to initial_map black_map pending pending0.
+    Local Transparent unallocated points_to initial_map black_map pending MapMS.pending.
 
     Lemma unallocated_alloc (sz: nat)
       :
-      unallocated sz -∗ (map_points_to sz 0 ∗ unallocated (Z.pos (Pos.of_succ_nat sz))).
+      unallocated sz -∗ (points_to sz 0 ∗ unallocated (Z.pos (Pos.of_succ_nat sz))).
     Proof.
-      unfold map_points_to, unallocated. iIntros "H".
-      replace (unallocated_r sz) with ((map_points_to_r sz 0) ⋅ (unallocated_r (S sz))).
+      unfold points_to, unallocated. iIntros "H".
+      replace (unallocated_r sz) with ((points_to_r sz 0) ⋅ (unallocated_r (S sz))).
       { ss. iDestruct "H" as "[H0 H1]". iFrame. }
-      unfold unallocated_r, map_points_to_r. ur. f_equal.
+      unfold unallocated_r, points_to_r. ur. f_equal.
       { ur. auto. }
       { ur. unfold Auth.white. f_equal. ur. extensionality k.
         ur. des_ifs; try by (exfalso; lia).
@@ -77,9 +79,9 @@ Section SIMMODSEM.
 
     Lemma initial_map_no_points_to k v
       :
-      initial_map -∗ map_points_to k v -∗ ⌜False⌝.
+      initial_map -∗ points_to k v -∗ ⌜False⌝.
     Proof.
-      unfold initial_map, map_points_to.
+      unfold initial_map, points_to.
       iIntros "H0 H1". iCombine "H0 H1" as "H".
       iOwnWf "H" as WF. exfalso. rr in WF. ur in WF. unseal "ra". des.
       rr in WF0. ur in WF0. unseal "ra". des.
@@ -89,9 +91,9 @@ Section SIMMODSEM.
 
     Lemma unallocated_range sz k v
       :
-      unallocated sz -∗ map_points_to k v -∗ ⌜(0 <= k < sz)%Z⌝.
+      unallocated sz -∗ points_to k v -∗ ⌜(0 <= k < sz)%Z⌝.
     Proof.
-      unfold unallocated, map_points_to.
+      unfold unallocated, points_to.
       iIntros "H0 H1". iCombine "H0 H1" as "H".
       iOwnWf "H" as WF. iPureIntro. rr in WF. ur in WF. unseal "ra". des.
       rr in WF. ur in WF0. unseal "ra".
@@ -101,9 +103,9 @@ Section SIMMODSEM.
 
     Lemma black_map_get f k v
       :
-      black_map f -∗ map_points_to k v -∗ (⌜f k = v⌝).
+      black_map f -∗ points_to k v -∗ (⌜f k = v⌝).
     Proof.
-      unfold black_map, map_points_to.
+      unfold black_map, points_to.
       iIntros "H0 H1". iCombine "H0 H1" as "H".
       iOwnWf "H" as WF. iPureIntro. rr in WF. ur in WF. unseal "ra". des.
       rr in WF0. ur in WF0. unseal "ra". des.
@@ -113,11 +115,11 @@ Section SIMMODSEM.
 
     Lemma black_map_set f k w v
       :
-      black_map f -∗ map_points_to k w -∗ #=> (black_map (<[k:=v]>f) ∗ map_points_to k v).
+      black_map f -∗ points_to k w -∗ #=> (black_map (<[k:=v]>f) ∗ points_to k v).
     Proof.
       iIntros "H0 H1". iCombine "H0 H1" as "H".
       iPoseProof (OwnM_Upd with "H") as "H".
-      { instantiate (1:=black_map_r (<[k:=v]>f) ⋅ map_points_to_r k v).
+      { instantiate (1:=black_map_r (<[k:=v]>f) ⋅ points_to_r k v).
         rr. intros ctx WF. ur in WF. ur. unseal "ra". des_ifs. des. split; auto.
         ur in WF0. ur. des_ifs. des. rr in WF0. des. split.
         { rr. exists ctx. ur in WF0. ur. extensionality n.
@@ -140,24 +142,26 @@ Section SIMMODSEM.
     
   End LEMMA.
 
-  Variable GlobalStb: Sk.t -> gname -> option fspec.
-  Hypothesis STB_set: forall sk, (GlobalStb sk) "set" = Some set_spec.
+  Variable StbA: Sk.t -> gname -> option fspec.
+  Hypothesis MapInStbA: forall sk, stb_incl (to_stb MapAS.Stb) (StbA sk).
 
-  Variable GlobalStbM: Sk.t -> gname -> option fspec.
-  Hypothesis STB_setM: forall sk, (GlobalStbM sk) "set" = Some set_specM.
-
+  Variable StbM: Sk.t -> gname -> option fspec.
+  Hypothesis MapInStbM: forall sk, stb_incl (to_stb MapMS.Stb) (StbM sk).
+  
   (* TODO: Try spawn & consume a dummy world *)
   Definition Ist: Any.t -> Any.t -> iProp :=
     (fun st_src st_tgt =>
-       ((pending0 ∗ initial_map ∗ ⌜st_src = (fun (_: Z) => 0%Z)↑ /\ st_tgt = (fun (_: Z) => 0%Z, 0%Z)↑⌝)
+       ((MapMS.pending ∗ initial_map ∗ ⌜st_src = (fun (_: Z) => 0%Z)↑ /\ st_tgt = (fun (_: Z) => 0%Z, 0%Z)↑⌝)
         ∨ 
         (pending ∗ ∃ f sz, ⌜st_src = f↑ /\ st_tgt = (f, sz)↑⌝ ∗ black_map f ∗ unallocated sz))%I).
 
+  Local Notation MapAMod := (MapA.t MapM.Sem.(SModSem.initial_cond) StbA).
+  Local Notation MapMMod := (MapM.t StbM).
+
   Lemma simF_init:
-    HModR.sim_fun
-      (MapA.HMap GlobalStb) (MapM.HMap GlobalStbM) Ist "init".
+    HModR.sim_fun MapAMod MapMMod Ist MapName.init.
   Proof.
-    simF_init MapA.HMap_unfold MapM.HMap_unfold MapM.initF initF.
+    simF_init MapA.unfold MapM.unfold MapA.init MapM.init.
 
     (* SRC: handle the IST of Map and the precond of init *)
     st_l. hss. iDestruct "ASM" as "(W & (%Y & %M & P) & %X)".
@@ -185,10 +189,9 @@ Section SIMMODSEM.
   Qed.
 
   Lemma simF_get:
-    HModR.sim_fun
-      (MapA.HMap GlobalStb) (MapM.HMap GlobalStbM) Ist "get".
+    HModR.sim_fun MapAMod MapMMod Ist MapName.get.
   Proof.
-    simF_init MapA.HMap_unfold MapM.HMap_unfold MapM.getF getF.
+    simF_init MapA.unfold MapM.unfold MapA.get MapM.get.
 
     (* SRC: handle the IST of Map and the precond of get *)
     st_l. hss. iDestruct "ASM" as "(WORLD & (% & MAP) & %)".
@@ -221,10 +224,9 @@ Section SIMMODSEM.
   Qed.
 
   Lemma simF_set:
-    HModR.sim_fun
-      (MapA.HMap GlobalStb) (MapM.HMap GlobalStbM) Ist "set".
+    HModR.sim_fun MapAMod MapMMod Ist MapName.set.
   Proof.
-    simF_init MapA.HMap_unfold MapM.HMap_unfold MapM.setF setF.
+    simF_init MapA.unfold MapM.unfold MapA.set MapM.set.
 
     (* SRC: handle the IST of Map and the precond of set *)
     st_l. hss. iDestruct "ASM" as "(WORLD & (% & MAP) & %)".
@@ -257,10 +259,9 @@ Section SIMMODSEM.
   Qed.
 
   Lemma simF_set_by_user:
-    HModR.sim_fun
-      (MapA.HMap GlobalStb) (MapM.HMap GlobalStbM) Ist "set_by_user".
+    HModR.sim_fun MapAMod MapMMod Ist MapName.set_by_user.
   Proof.
-    simF_init MapA.HMap_unfold MapM.HMap_unfold MapM.set_by_userF set_by_userF.
+    simF_init MapA.unfold MapM.unfold MapA.set_by_user MapM.set_by_user.
 
     (* SRC: handle the IST of Map and the precond of set_by_user *)
     st_l. hss. iDestruct "ASM" as "(WORLD & (% & MAP) & %)".
@@ -275,11 +276,13 @@ Section SIMMODSEM.
     st_r. st. hss.
 
     (* TGT: handle the precond of set *)
-    rewrite STB_setM in G. hss. rewrite !HoareCall_parse. unfold HoareCallPre.
+    unfold_stb MapInStbM MapMS.Stb. i; hss.
+    rewrite !HoareCall_parse. unfold HoareCallPre.
     st_r. iDestruct "GRT" as "[[WORLD [% %]] _]". subst. hss.
 
     (* SRC: prove the precond of set *)
-    rewrite STB_set. st_l. rewrite !HoareCall_parse. unfold HoareCallPre.
+    unfold_stb MapInStbA MapAS.Stb.
+    st_l. rewrite !HoareCall_parse. unfold HoareCallPre.
     st_l. force_l. instantiate (1:= mk_meta _ _ (_,_,_)).
     force_l. force_l.
     iSplitL "WORLD MAP". { iFrame. eauto. }
@@ -307,7 +310,7 @@ Section SIMMODSEM.
     st. eauto.
   Qed.
   
-  Theorem sim: HModR.sim (MapA.HMap GlobalStb) (MapM.HMap GlobalStbM) Ist.
+  Theorem sim: HModR.sim MapAMod MapMMod Ist.
   Proof.
     sim_init.
     - iIntros "(IST & P & INIT0)"; s. iSplitL "INIT0"; eauto.
