examples/map/MapMSpec.v
@@ -1,0 +1,77 @@
+Require Import Coqlib ITreelib sflib.
+Require Import ImpPrelude.
+Require Import Events STS.
+Require Import Behavior.
+Require Import HMod SMod.
+Require Import Skeleton.
+Require Import PCM IPM STB.
+From ExtLib Require Import
+     Core.RelDec
+     Structures.Maps
+     Data.Map.FMapAList.
+Require Import ISim.
+Require Import MapHeader Mem1.
+Require Import sProp sWorld World SRF.
+From stdpp Require Import coPset gmap namespaces.
+Set Implicit Arguments.
+
+Module MapMS.
+Section MAP.
+  Context `{_W: CtxWD.t}.
+
+  Definition RA: URA.t := Excl.t unit.
+  Context `{@GRA.inG RA Γ}. 
+
+  Definition pending_r: RA := Excl.just tt.
+
+  Definition pending: iProp :=
+    OwnM pending_r.
+
+  Global Opaque pending.
+
+  Definition init_spec: fspec :=
+    mk_fspec_inv 0
+      (fun _ _ => mk_simple (fun (sz: nat) =>
+                    (ord_top,
+                      (fun varg => (⌜varg = ([Vint sz]: list val)↑⌝
+                                     ∗ ⌜(8 * (Z.of_nat sz) < modulus_64%Z)%Z⌝
+                                     ∗ pending)%I),
+                      (fun vret => True%I)))).
+
+  Definition get_spec: fspec := 
+    mk_fspec_inv 0
+    (fun _ _ => mk_simple (fun k =>
+                  (ord_top,
+                    (fun varg => (⌜varg = ([Vint k])↑⌝)%I),
+                    (fun vret => True%I)))).  
+
+  Definition set_spec: fspec :=
+    mk_fspec_inv 0
+    (fun _ _ => mk_simple (fun '(k, v) =>
+                  (ord_top,
+                    (fun varg => (⌜varg = ([Vint k; Vint v])↑⌝)%I),
+                    (fun vret => True%I)))).  
+
+  Definition set_by_user_spec: fspec := 
+    mk_fspec_inv 0
+    (fun _ _ => mk_simple (fun k =>
+                  (ord_top,
+                    (fun varg => (⌜varg = ([Vint k])↑⌝)%I),
+                    (fun vret => True%I)))).  
+
+  Definition Stb: alist gname fspec :=
+    Seal.sealing "stb" [(MapName.init, init_spec);
+                        (MapName.get, get_spec);
+                        (MapName.set, set_spec);
+                        (MapName.set_by_user, set_by_user_spec)].
+
+End MAP.
+End MapMS.
+
+Module MapMR.
+  Class t
+    `{@GRA.inG MapMS.RA Γ}
+    := MapRA: unit.
+
+End MapMR.
+
